

1. Use the Chain Rule to find  $\frac{\partial w}{\partial s}$  and  $\frac{\partial w}{\partial t}$  for

$$w = xyz, \quad x = s + t, \quad y = s - t, \quad z = st^2$$

**Solution:** Note that

$$\begin{array}{lll} \frac{\partial w}{\partial x} = yz & \frac{\partial w}{\partial y} = xz & \frac{\partial w}{\partial z} = xy \\ \frac{\partial x}{\partial s} = 1 & \frac{\partial y}{\partial s} = 1 & \frac{\partial z}{\partial s} = t^2 \\ \frac{\partial x}{\partial t} = 1 & \frac{\partial y}{\partial t} = -1 & \frac{\partial z}{\partial t} = 2st \end{array}$$

and so

$$\begin{aligned} \frac{\partial w}{\partial s} &= \frac{\partial w}{\partial x} \frac{\partial x}{\partial s} + \frac{\partial w}{\partial y} \frac{\partial y}{\partial s} + \frac{\partial w}{\partial z} \frac{\partial z}{\partial s} \\ &= (yz)(1) + (xz)(1) + (xy)(t^2) \\ &= yz + xz + t^2xy \\[1em] \frac{\partial w}{\partial t} &= \frac{\partial w}{\partial x} \frac{\partial x}{\partial t} + \frac{\partial w}{\partial y} \frac{\partial y}{\partial t} + \frac{\partial w}{\partial z} \frac{\partial z}{\partial t} \\ &= (yz)(1) + (xz)(-1) + (xy)(2st) \\ &= yz - xz + 2stxy \end{aligned}$$

2. Differentiate implicitly to find the first partial derivatives of  $z$  for

$$e^{xz} + xy = 0$$

**Solution:** Since  $f(x, y, z) = e^{xz} + xy = 0$  and

$$F_x(x, y, z) = e^{xz} + y$$

$$F_y(x, y, z) = x$$

$$F_z(x, y, z) = e^{xz}$$

we note that  $F_z(x, y, z) = e^{xz} \neq 0$  then

$$\frac{\partial z}{\partial x} = -\frac{F_x(x, y, z)}{F_z(x, y, z)} = -\frac{e^{xz} + y}{e^{xz}}$$

$$\frac{\partial z}{\partial y} = -\frac{F_y(x, y, z)}{F_z(x, y, z)} = -\frac{x}{e^{xz}}$$

3. If  $z = 5x^2 + y^2$  and  $(x, y)$  changes from  $(1, 2)$  to  $(1.05, 2.1)$ , compare the values of  $\Delta z$  and  $dz$ .

**Solution:** Let  $(x, y) = (1, 2)$  then  $(x + \Delta x, y + \Delta y) = (1.05, 2.1)$ . This means that

$$dx = \Delta x = 0.05 \qquad dy = \Delta y = 0.1$$

so the differential is given by

$$\Delta z \approx dz = \frac{\partial z}{\partial x} dx + \frac{\partial z}{\partial y} dy = 10x dx + 2y dy$$

when  $(x, y) = (1, 2)$  then

$$\Delta z \approx 10(1)(0.05) + 2(2)(0.1) = 0.9$$

for the actual change in  $z$  we have

$$\begin{aligned} \Delta z &= f(1.05, 2.1) - f(1, 2) \\ &= 5(1.05)^2 + (2.1)^2 - (5(1)^2 + (2)^2) \\ &= 9.9225 - 9 = 0.9225 \end{aligned}$$

4. Compute  $\frac{\partial g}{\partial s}$  at  $(t, s) = (1, 2)$  if

$$g(x, y) = x^2 - y^2, \quad x = t^2 + s^2, \quad y = t^3 - 2s$$

**Solution:** Since  $x$  and  $y$  are functions of  $t$  and  $s$ , then  $g(x, y)$  is a function of two independent variables,  $t$  and  $s$  i.e  $g(x(t, s), y(t, s))$ . The appropriate version of the chain rule is

$$\frac{\partial g}{\partial s} = \frac{\partial g}{\partial x} \frac{\partial x}{\partial s} + \frac{\partial g}{\partial y} \frac{\partial y}{\partial s}$$

Since

$$\frac{\partial g}{\partial x} = 2x, \quad \frac{\partial g}{\partial y} = -2y$$

$$\frac{\partial x}{\partial s} = 2s, \quad \frac{\partial y}{\partial s} = -2$$

and so

$$\frac{\partial g}{\partial s} = 4xs + 4y$$

When  $(t, s) = (1, 2)$  we see that

$$x(1, 2) = (1)^2 + (2)^2 = 5 \quad \text{and} \quad y(1, 2) = (1)^3 - 2(2) = -3$$

then

$$\begin{aligned} \frac{\partial g}{\partial s}(1, 2) &= 4(5)(2) + 4(-3) \\ &= 40 - 12 \\ &= 28. \end{aligned}$$